Iterator/Lemmas/Consumer.lean
@@ -1,6 +1,7 @@
-import Iterator.Producers
 import Iterator.Consumers
 import Iterator.Combinators.FilterMap
+import Iterator.Lemmas.Equivalence
+import Iterator.Producers
 
 section Consumers
 
@@ -134,6 +135,7 @@ theorem Iter.reverseToList_of_step [Monad m] [LawfulMonad m] [Iterator α m β] 
   obtain ⟨step, h⟩ := step
   cases step <;> simp [Iter.reverseToList.go.aux₂]
 
+-- TODO: rename `reverseToList` -> `toListRev`
 theorem Iter.reverse_reverseToList [Monad m] [LawfulMonad m] [Iterator α m β]
     [IteratorToArray α m] [LawfulIteratorToArray α m]
     {it : Iter (α := α) m β} :
@@ -148,151 +150,41 @@ theorem Iter.reverse_reverseToList [Monad m] [LawfulMonad m] [Iterator α m β]
 
 end Consumers
 
-section ListIterator
+section Congruence
 
-variable {m : Type v → Type v} [Monad m] {β : Type v}
+theorem Iter.Morphism.toArrayMapped_eq {α α' : Type w} {m : Type w → Type w'}
+    {β : Type v} {γ : Type w}
+    [Monad m] [LawfulMonad m]
+    [Iterator α m β] [Iterator α' m β] [IteratorToArray α m] [LawfulIteratorToArray α m]
+    [IteratorToArray α' m] [LawfulIteratorToArray α' m]
+    (φ : Morphism α α' m) {f : β → m γ} {it : Iter (α := α) m β} :
+    IteratorToArray.toArrayMapped f it = IteratorToArray.toArrayMapped f (φ.map it) := by
+  haveI : Finite α m := LawfulIteratorToArray.finite
+  haveI : Finite α' m := LawfulIteratorToArray.finite
+  simp only [LawfulIteratorToArray.lawful]
+  induction it using Iter.induct with | step it ihy ihs =>
+  rw [DefaultConsumers.toArrayMapped_of_stepH, DefaultConsumers.toArrayMapped_of_stepH]
+  simp only [← φ.stepH_hom, map_eq_pure_bind, bind_assoc]
+  apply bind_congr
+  intro step
+  generalize step.inflate = step
+  obtain ⟨step, _⟩ := step
+  cases step <;> simp (discharger := assumption) [PlausibilityMorphism.mapStep, IterStep.map, ihs, ihy]
 
--- theorem List.step_iter_nil :
---     (([] : List β).iter m).step = pure ⟨.done, .done, sorry, [], sorry⟩
+theorem Iter.Morphism.toArray_eq {α α' : Type w} {m : Type w → Type w'} {β : Type w}
+    [Monad m] [LawfulMonad m]
+    [Iterator α m β] [Iterator α' m β] [IteratorToArray α m] [LawfulIteratorToArray α m]
+    [IteratorToArray α' m] [LawfulIteratorToArray α' m]
+    (φ : Morphism α α' m) {it : Iter (α := α) m β} :
+    it.toArray = (φ.map it).toArray := by
+  simp [Iter.toArray, φ.toArrayMapped_eq]
 
--- private theorem List.toArray_iter.aux {l : List β} {acc : Array β} :
---     Iter.toArray.go (l.iter m) acc = pure (acc ++ l.toArray) := by
---   simp [List.iter]
---   induction l generalizing acc with
---   | nil =>
---     rw [Iter.toArray.go]
---     simp [Iter.step, Iter.stepH, CodensityT.run, CodensityT.mapH, Iterator.step,
---       IterationT.map_eq_mapH, IterationT.mapH, IterationT.computation_pure, Pure.pure]
---     simp [Iter.Step.ofInternal, IterationT.Plausible.map, IterStep.map]
---   | cons x xs ih =>
---     rw [Iter.toArray.go]
---     simp [Iter.step, Iter.stepH, CodensityT.run, CodensityT.mapH, Iterator.step,
---       IterationT.map_eq_mapH, IterationT.mapH, IterationT.computation_pure, Pure.pure,
---       Iter.Step.ofInternal, IterationT.Plausible.map, IterStep.map, ih]
+theorem Iter.Morphism.toList_eq {α α' : Type w} {m : Type w → Type w'} {β : Type w}
+    [Monad m] [LawfulMonad m]
+    [Iterator α m β] [Iterator α' m β] [IteratorToArray α m] [LawfulIteratorToArray α m]
+    [IteratorToArray α' m] [LawfulIteratorToArray α' m]
+    (φ : Morphism α α' m) {it : Iter (α := α) m β} :
+    it.toList = (φ.map it).toList := by
+  simp [← Iter.toList_toArray, φ.toArray_eq]
 
--- private theorem List.toArray_iter {l : List β} :
---     Iter.toArray (l.iter m)
-
-end ListIterator
-
--- section Equivalence
-
--- variable {α : Type u} {m : Type w → Type w'} {β : Type v}
-
--- inductive IterTStep (β : Type v) where
---   | yield : β → IterTStep β
---   | skip : IterTStep β
---   | done : IterTStep β
-
--- inductive IterT (m : Type w → Type w') (β : Type v) : Type w → Type (max v w w' + 1) where
---   | step : ∀ {α}, Nat → (β → α) → IterT m β (IterTStep α)
---   | lift : ∀ {α}, m α → IterT m β α
---   | bind : ∀ {α γ}, IterT m β α → (α → IterT m β γ) → IterT m β γ
-
--- def IterT.interpret [Iterator α m β] [Monad m] (it : α) (γ : Type w) (x : IterT m β γ) : m γ :=
---   go [it] x |>.mapH (fun p => p.1) |>.run
--- where
---   go {δ : Type w} (its : List α) : IterT m β δ → CodensityT m (δ × List α)
---     | .step n f => match its[n]? with
---       | none => pure (.done, its)
---       | some it =>
---         let v := Iterator.step it
---         v.mapH (match · with
---           | .yield it' out _ => (.yield (f out), it' :: its)
---           | .skip it' _ => (.skip, it' :: its)
---           | .done _ => (.done, its))
---     | .lift x => (CodensityT.eval x).mapH (Prod.mk · its)
---     | .bind x f => (go its x) >>= (fun y => go y.2 (f y.1))
-
--- end Equivalence
-
--- variable {α : Type u} {m : Type w → Type w'} {β : Type v}
---   [Iterator α m β] {_ : ComputableSmall.{w} α} (it : Iter (α := α) m β)
---   [Monad m]
---   (f : β → CodensityT m (Option β'))
-
--- theorem FilterMapMH.plausible_of_yield_of_none {it' : Iter (α := α) m β} {out : β}
---     (h : it.plausible_step (.yield it' out)) :
---     (it.filterMapMH f).plausible_step (.skip (it'.filterMapMH f)) := by
---   let step : it.Step := .yield it' out h
---   let internalStep := step.toInternal
---   simp only [Iter.plausible_step]
---   refine ⟨.skip (it'.filterMapMH f).inner, by simp [IterStep.map, Iter.filterMapMH], ?_⟩
---   refine ⟨.yield (it'.filterMapMH f).inner.inner out, ?_, ?_⟩
---   · exact ⟨none, rfl, True.intro⟩
---   · simp only [Iter.filterMapMH, Iterator.filterMapMH, inner_toIter]
---     exact internalStep.property
-
--- theorem FilterMapMH.plausible_of_yield_of_some {it' : Iter (α := α) m β} {out : β} {out' : β'}
---     (h : it.plausible_step (.yield it' out)) :
---     (it.filterMapMH f).plausible_step (.yield (it'.filterMapMH f) out') := by
---   let step : it.Step := .yield it' out h
---   let internalStep := step.toInternal
---   refine ⟨.yield (it'.filterMapMH f).inner out', by simp [IterStep.map, Iter.filterMapMH], ?_⟩
---   refine ⟨.yield (it'.filterMapMH f).inner.inner out, ?_, ?_⟩
---   · exact ⟨some out', rfl, True.intro⟩
---   · simp only [Iter.filterMapMH, Iterator.filterMapMH, inner_toIter]
---     exact internalStep.property
-
--- theorem FilterMapMH.plausible_of_skip {it' : Iter (α := α) m β}
---     (h : it.plausible_step (.skip it')) :
---     (it.filterMapMH f).plausible_step (.skip (it'.filterMapMH f)) := by
---   let step : it.Step := .skip it' h
---   let internalStep := step.toInternal
---   refine ⟨.skip (it'.filterMapMH f).inner, by simp [IterStep.map, Iter.filterMapMH], ?_⟩
---   refine ⟨.skip (it'.filterMapMH f).inner.inner, rfl, ?_⟩
---   simp only [Iter.filterMapMH, Iterator.filterMapMH, inner_toIter]
---   exact internalStep.property
-
--- theorem FilterMapMH.plausible_of_done
---     (h : it.plausible_step .done) :
---     (it.filterMapMH f).plausible_step .done := by
---   let step : it.Step := .done h
---   let internalStep := step.toInternal
---   refine ⟨.done, by simp [IterStep.map, Iter.filterMapMH], ?_⟩
---   refine ⟨.done, rfl, ?_⟩
---   simp only [Iter.filterMapMH, Iterator.filterMapMH, inner_toIter]
---   exact internalStep.property
-
--- theorem filterMapMH_step :
---   (it.filterMapMH f).stepH = (it.stepH.bindH (match · with
---       | .yield it' out h => (f out).mapH fun
---           | none => .skip (it'.filterMapMH f) (FilterMapMH.plausible_of_yield_of_none _ _ h)
---           | some out' => .yield (it'.filterMapMH f) out' (FilterMapMH.plausible_of_yield_of_some _ _ h)
---       | .skip it' h => pure <| .skip (it'.filterMapMH f) (FilterMapMH.plausible_of_skip _ _ h)
---       | .done h => pure <| .done (FilterMapMH.plausible_of_done _ _ h))) := by
---   cases it
---   simp only [Iter.filterMapMH, Iterator.filterMapMH]
---   rw [Iter.stepH, CodensityT.mapH_eq_bindH]
---   rw [Iter.stepH, CodensityT.mapH_eq_bindH]
---   simp only [plausible_eq_copy
---     (congrArg Iterator.step (inner_toIter ..)),
---     congrArg Iterator.step, congrArg FilterMapMH.inner, inner_toIter]
---   simp only [Iterator.step]
---   rw [CodensityT.map_eq_mapH, CodensityT.mapH_eq_bindH]
---   simp only [IterationT.bindH]
---   simp only [CodensityT.bindH_assoc]
---   refine congrArg (CodensityT.bindH _ ·) ?_
---   ext x
---   simp only [CodensityT.bindH_pure, Iter.Step.ofInternal, IterationT.Plausible.map, IterStep.map]
---   match h : x with
---   | ⟨.yield .., h⟩ =>
---     simp only [matchStep]
---     simp only [IterationT.mapH, CodensityT.mapH_eq_bindH, monadLift, MonadLift.monadLift,
---       CodensityT.map_eq_mapH, CodensityT.mapH_eq_bindH, CodensityT.bindH_assoc,
---       CodensityT.bindH_pure]
---     refine congrArg (CodensityT.bindH _ ·) ?_
---     ext y
---     refine congrArg pure ?_
---     simp only [IterationT.Plausible.copy, Iter.Step.yield, Iter.Step.skip, Iter.filterMapMH,
---       Iterator.filterMapMH, inner_toIter]
---     cases y <;> rfl
---   | ⟨.skip .., h⟩ =>
---     simp only [matchStep]
---     simp only [CodensityT.mapH_eq_bindH, IterationT.computation_pure, CodensityT.bindH_pure,
---       IterationT.Plausible.copy, Iter.Step.skip, Iter.filterMapMH, Iterator.filterMapMH,
---       inner_toIter]
---   | ⟨.done, h⟩ =>
---     simp only [matchStep, IterationT.Plausible.copy, CodensityT.mapH_eq_bindH, CodensityT.bindH_assoc,
---       IterationT.computation_pure, CodensityT.bindH_pure]
---     rfl
+end Congruence
