Iterator/Lemmas/Equivalence.lean
@@ -1,0 +1,34 @@
+import Iterator.Basic
+
+structure Iter.PlausibilityMorphism (α α' : Type w) (m : Type w → Type w') {β : Type v}
+    [Iterator α m β] [Iterator α' m β] where
+  map : Iter (α := α) m β → Iter (α := α') m β
+  plausible_step_map : ∀ {it : Iter (α := α) m β} {step : IterStep (Iter (α := α) m β) β},
+      (map it).plausible_step (step.map map id) ↔ it.plausible_step step
+
+def Iter.PlausibilityMorphism.mapStep {α α' : Type w} {m : Type w → Type w'} {β : Type v}
+    [Iterator α m β] [Iterator α' m β] (φ : PlausibilityMorphism α α' m)
+    {it : Iter (α := α) m β} (step : it.Step) : (φ.map it).Step :=
+  ⟨step.1.map φ.map id, φ.plausible_step_map.mpr step.2⟩
+
+structure Iter.Morphism (α α' : Type w) (m : Type w → Type w') [Functor m] {β : Type v}
+    [Iterator α m β] [Iterator α' m β] extends Iter.PlausibilityMorphism α α' m where
+  stepH_hom : ∀ {it : Iter (α := α) m β},
+      (.deflate <| toPlausibilityMorphism.mapStep ·.inflate) <$> it.stepH = (map it).stepH
+
+def Iter.Morphism.id (α : Type w) (m : Type w → Type w') [Functor m] [LawfulFunctor m] {β : Type v} [Iterator α m β] :
+    Morphism α α m where
+  map it := it
+  plausible_step_map {it step} := by
+    change it.plausible_step (step.map _root_.id _root_.id) ↔ it.plausible_step step
+    simp [IterStep.map_id]
+  stepH_hom {it} := by
+    simp only [PlausibilityMorphism.mapStep]
+    conv => rhs; rw [← id_map (x := it.stepH)]
+    refine congrArg (· <$> _) ?_
+    ext step
+    conv => rhs; rw [← USquash.deflate_inflate (x := step)]
+    refine congrArg USquash.deflate ?_
+    generalize step.inflate = step
+    obtain ⟨step, _⟩ := step
+    cases step <;> simp
